Move things into their own files, start WP calculus. FIXME: create makefile!

lang.v
@@ -5,286 +5,136 @@ Require Import String ZArith Lia.
 Open Scope string_scope.
 Open Scope Z_scope.
 
-Section Lang.
+Declare Scope lang_scope.
 
-  Declare Scope lang_scope.
+Inductive binop := Add | Sub | Leq.
 
-  Inductive binop := Add | Sub | Leq.
+Inductive expr : Type :=
+| Var : string -> expr
+| Const : Z -> expr
+| Binop : binop -> expr -> expr -> expr.
 
-  Inductive expr : Type :=
-  | Var : string -> expr
-  | Const : Z -> expr
-  | Binop : binop -> expr -> expr -> expr.
+Inductive insn : Type :=
+| Skip : insn
+| Assign : string -> expr -> insn
+| Seq : insn -> insn -> insn
+| Ite : expr -> insn -> insn -> insn
+| While : expr -> insn -> insn.
 
-  Inductive insn : Type :=
-  | Skip : insn
-  | Assign : string -> expr -> insn
-  | Seq : insn -> insn -> insn
-  | Ite : expr -> insn -> insn -> insn
-  | While : expr -> insn -> insn.
+Coercion Var : string >-> expr.
+Coercion Const : Z >-> expr.
 
-  Coercion Var : string >-> expr.
-  Coercion Const : Z >-> expr.
+Infix "+" := (Binop Add) : lang_scope.
+Infix "-" := (Binop Sub) : lang_scope.
+Infix "<=" := (Binop Leq)(at level 70) : lang_scope.
 
-  Infix "+" := (Binop Add) : lang_scope.
-  Infix "-" := (Binop Sub) : lang_scope.
-  Infix "<=" := (Binop Leq)(at level 70) : lang_scope.
+Open Scope lang_scope.
+Check "foo" + 3.
 
-  Open Scope lang_scope.
-  Check "foo" + 3.
+Notation "x :== e" := (Assign x e) (at level 80) : lang_scope.
+Infix ";" := Seq (at level 90, right associativity) : lang_scope.
+Notation "'If' e 'Then' i 'Else' j" := (Ite e i j)(at level 95) : lang_scope.
 
-  Notation "x :== e" := (Assign x e) (at level 80) : lang_scope.
-  Infix ";" := Seq (at level 90, right associativity) : lang_scope.
-  Notation "'If' e 'Then' i 'Else' j" := (Ite e i j)(at level 95) : lang_scope.
+Check (If 3 Then Skip Else Skip).
 
-  Check (If 3 Then Skip Else Skip).
+Notation "'While' e 'Do' i 'Done'" := (While e i)(at level 100) : lang_scope.
 
-  Notation "'While' e 'Do' i 'Done'" := (While e i)(at level 100) : lang_scope.
+Check (While "x" <= 10 Do "x" :== "x" + 1; "y" :== "y" - 1; Skip Done).
 
-  Check (While "x" <= 10 Do "x" :== "x" + 1; "y" :== "y" - 1; Skip Done).
+Definition env := string -> Z.
 
-  Definition env := string -> Z.
+Definition equiv_env (f g : env) : Prop := forall s, f s = g s.
 
-  Definition equiv_env (f g : env) : Prop := forall s, f s = g s.
- 
-  Notation "f ≃ g" := (equiv_env f g)(at level 50).
+Notation "f ≃ g" := (equiv_env f g)(at level 50).
 
-  Search (Z -> Z -> bool).
-  
-  Definition eval_op (o : binop) : Z -> Z -> Z :=
-    match o with
-    | Add => Z.add
-    | Sub => Z.sub
-    | Leq => (fun x y => if Z.leb x y then 1 else 0)
-    end.
-  
-  Fixpoint eval_expr (f : env) (e : expr) : Z :=
-    match e with
-    | Var v => f v
-    | Const c => c
-    | Binop o e1 e2 => eval_op o (eval_expr f e1) (eval_expr f e2)
-    end.
+Search (Z -> Z -> bool).
 
-  Eval compute in (eval_expr (fun _ => 0) ("x" + "y" + 2 - 1)).
+Definition eval_op (o : binop) : Z -> Z -> Z :=
+  match o with
+  | Add => Z.add
+  | Sub => Z.sub
+  | Leq => (fun x y => if Z.leb x y then 1 else 0)
+  end.
 
-  Search (string -> string -> bool).
+Fixpoint eval_expr (f : env) (e : expr) : Z :=
+  match e with
+  | Var v => f v
+  | Const c => c
+  | Binop o e1 e2 => eval_op o (eval_expr f e1) (eval_expr f e2)
+  end.
 
-  Check String.eqb.
-  Search (eqb).
+Eval compute in (eval_expr (fun _ => 0) ("x" + "y" + 2 - 1)).
 
-  Definition by_cases (f : env) (x : string) (v : Z) : env :=
-    fun y => if String.eqb x y then v else f y.
+Search (string -> string -> bool).
 
-  Hint Unfold by_cases.
+Check String.eqb.
+Search (eqb).
 
-  Notation "f [ x --> v ]" := (by_cases f x v)(at level 70).
-  
-  Inductive big_step : env -> insn -> env -> Prop :=
-  | BS_Skip : forall f,
-      big_step f Skip f
-  | BS_Assign : forall f x e v,
-      eval_expr f e = v ->
-      big_step f (x :== e) (f[x --> v])
-  | BS_Seq : forall f g h i j,
-      big_step f i g ->
-      big_step g j h ->
-      big_step f (i;j) h
-  | BS_Ite_true : forall f g e i j,
-      big_step f i g ->
-      eval_expr f e <> 0 ->
-      big_step f (If e Then i Else j) g
-  | BS_Ite_false : forall f g e i j,
-      big_step f j g ->
-      eval_expr f e = 0 ->
-      big_step f (If e Then i Else j) g
-  | BS_While_halt : forall f e i,
-      eval_expr f e = 0 ->
-      big_step f (While e Do i Done) f
-  | BS_While_continue : forall f g h e i,
-      eval_expr f e <> 0 ->
-      big_step f i g ->
-      big_step g (While e Do i Done) h ->
-      big_step f (While e Do i Done) h.
+Definition by_cases (f : env) (x : string) (v : Z) : env :=
+  fun y => if String.eqb x y then v else f y.
 
-  Locate "≃".
+Hint Unfold by_cases.
 
-  Hint Constructors big_step.
+Notation "f [ x --> v ]" := (by_cases f x v)(at level 70).
 
-  Lemma eval_ext : forall e (f f' : env),
-      f ≃ f' -> eval_expr f e = eval_expr f' e.
-  Proof.
-    unfold equiv_env; intros; induction e; simpl; auto.
-    erewrite IHe1; erewrite IHe2; now auto.
-  Qed.
+Inductive big_step : env -> insn -> env -> Prop :=
+| BS_Skip : forall f,
+    big_step f Skip f
+| BS_Assign : forall f x e v,
+    eval_expr f e = v ->
+    big_step f (x :== e) (f[x --> v])
+| BS_Seq : forall f g h i j,
+    big_step f i g ->
+    big_step g j h ->
+    big_step f (i;j) h
+| BS_Ite_true : forall f g e i j,
+    big_step f i g ->
+    eval_expr f e <> 0 ->
+    big_step f (If e Then i Else j) g
+| BS_Ite_false : forall f g e i j,
+    big_step f j g ->
+    eval_expr f e = 0 ->
+    big_step f (If e Then i Else j) g
+| BS_While_halt : forall f e i,
+    eval_expr f e = 0 ->
+    big_step f (While e Do i Done) f
+| BS_While_continue : forall f g h e i,
+    eval_expr f e <> 0 ->
+    big_step f i g ->
+    big_step g (While e Do i Done) h ->
+    big_step f (While e Do i Done) h.
 
-  Hint Rewrite eval_ext.
+Locate "≃".
 
-  (* It's nice to know evaluation is deterministic... *)
-  Theorem big_step_ext : forall (i : insn) (f g : env),
-      big_step f i g ->
-      forall i' f' g', big_step f' i' g' -> f ≃ f' -> i = i' -> g ≃ g'.
-  Proof.
-    intros i f g h1; induction h1; intros i' f' g' h2; induction h2; try (intros _ eq; now inversion eq); auto.
-    - unfold by_cases; intros f_eq i_eq; inversion i_eq; subst
-      ; intro y; try destruct (x0 =? y)%string; simpl; auto.
-      erewrite eval_ext; now auto.
-    - intros f_eq i_eq; eapply IHh1_2; eauto; [eapply IHh1_1; eauto; congruence| congruence].
-    - intros f_eq i_eq; eapply IHh1; eauto; congruence.
-    - intros f_eq i_eq; exfalso; apply H; erewrite eval_ext; eauto; congruence.
-    - intros f_eq i_eq; exfalso; apply H0; inversion i_eq; subst; erewrite eval_ext; eauto; intro; now auto.
-    - intros f_eq i_eq; eapply IHh1; eauto; congruence.
-    - intros f_eq i_eq; exfalso; apply H0; inversion i_eq; subst; erewrite eval_ext; eauto; intro; now auto.
-    - intros f_eq i_eq; exfalso; apply H; erewrite eval_ext; eauto; congruence.
-    - intros f_eq i_eq.
-      eapply IHh1_2; [ now eauto| | now eauto].
-      eapply IHh1_1; eauto; congruence.
-  Qed.
+Hint Constructors big_step.
 
-  Definition pred := env -> Prop.
+Lemma eval_ext : forall e (f f' : env),
+    f ≃ f' -> eval_expr f e = eval_expr f' e.
+Proof.
+  unfold equiv_env; intros; induction e; simpl; auto.
+  erewrite IHe1; erewrite IHe2; now auto.
+Qed.
 
-  (* Extraordinalriy awkward because of higher-order unification...
-     I think this is mostly solved by defining a WP.
-   *)
-  Inductive hoare : pred -> insn -> pred -> Prop :=
-  | H_Skip : forall P,
-      hoare P Skip P
-  | H_Assign : forall P x e,
-      hoare (fun f => P (f [x --> eval_expr f e])) (x :== e) P
-  | H_Seq : forall P Q R i j,
-      hoare P i Q ->
-      hoare Q j R ->
-      hoare P (i;j) R
-  | H_Ite : forall P Q e i j,
-      hoare (fun f => eval_expr f e <> 0 /\ P f) i Q ->
-      hoare (fun f => eval_expr f e = 0 /\ P f) j Q ->
-      hoare P (If e Then i Else j) Q
-  | H_While : forall (P Q I : pred) e i,
-      hoare (fun f => eval_expr f e <> 0 /\ I f) i I ->
-      (forall f, I f -> eval_expr f e = 0 -> Q f) ->
-      (forall f, P f -> I f) ->
-      hoare P (While e Do i Done) Q
-  | H_Weak : forall (P P' Q Q' : pred) i,
-      (forall f, P' f -> P f) ->
-      (forall f, Q f -> Q' f) ->
-      hoare P i Q ->
-      hoare P' i Q'
-  .
+Hint Rewrite eval_ext.
 
-  Hint Constructors hoare.
-  
-  Example test : hoare (fun f => True) ("foo" :== 42) (fun f => f "foo" = 42).
-  Proof.
-    eapply H_Weak.
-    - intros.
-      assert (H' : f ["foo" --> eval_expr f 42] "foo" = 42) by reflexivity.
-      exact H'.
-    - intros.
-      exact H.
-    - apply H_Assign with (P := fun f => f "foo" = 42).
-  Qed.
+(* It's nice to know evaluation is deterministic... *)
+Theorem big_step_ext : forall (i : insn) (f g : env),
+    big_step f i g ->
+    forall i' f' g', big_step f' i' g' -> f ≃ f' -> i = i' -> g ≃ g'.
+Proof.
+  intros i f g h1; induction h1; intros i' f' g' h2; induction h2; try (intros _ eq; now inversion eq); auto.
+  - unfold by_cases; intros f_eq i_eq; inversion i_eq; subst
+    ; intro y; try destruct (x0 =? y)%string; simpl; auto.
+    erewrite eval_ext; now auto.
+  - intros f_eq i_eq; eapply IHh1_2; eauto; [eapply IHh1_1; eauto; congruence| congruence].
+  - intros f_eq i_eq; eapply IHh1; eauto; congruence.
+  - intros f_eq i_eq; exfalso; apply H; erewrite eval_ext; eauto; congruence.
+  - intros f_eq i_eq; exfalso; apply H0; inversion i_eq; subst; erewrite eval_ext; eauto; intro; now auto.
+  - intros f_eq i_eq; eapply IHh1; eauto; congruence.
+  - intros f_eq i_eq; exfalso; apply H0; inversion i_eq; subst; erewrite eval_ext; eauto; intro; now auto.
+  - intros f_eq i_eq; exfalso; apply H; erewrite eval_ext; eauto; congruence.
+  - intros f_eq i_eq.
+    eapply IHh1_2; [ now eauto| | now eauto].
+    eapply IHh1_1; eauto; congruence.
+Qed.
 
-  Example test' : hoare (fun f => True) (If 0 Then Skip Else "foo" :== 42) (fun f => f "foo" = 42).
-  Proof.
-    apply H_Ite.
-    - simpl.
-      apply H_Weak with (P := fun f => f "foo" = 42)(Q := fun f => f "foo" = 42); intros; firstorder.
-    - eapply H_Weak with (P := fun f => f ["foo" --> eval_expr f 42] "foo" = 42)
-                         (Q := fun f => f "foo" = 42).
-      + simpl; now auto.
-      + now auto.
-      + apply H_Assign with (P := fun f => f "foo" = 42).
-  Qed.
-
-  Lemma while_inv : forall (I G : pred) i body f g e,
-      (forall f' g', I f' -> eval_expr f' e <> 0 -> big_step f' body g' -> I g') ->
-      (forall f', I f' -> eval_expr f' e = 0 -> G f') ->
-      I f ->
-      big_step f i g ->
-      (i = While e Do body Done) ->
-      G g.
-  Proof.
-    intros I G i body f g e inv_body inv_break init big.
-    induction big; intro eq; try inversion eq; subst; auto.
-    apply IHbig2; [| now auto].
-    eapply inv_body; [| apply H | apply big1].
-    apply init.
-  Qed.
-        
-  Theorem hoare_sound : forall f g P Q i,
-      hoare P i Q -> big_step f i g -> P f -> Q g.
-  Proof.
-    intros f g P Q i h.
-    revert f g.
-    induction h; intros f g step; inversion step; subst; eauto.
-    (* 1 subgoal! *)
-    intro hf.
-    eapply while_inv; intros.
-    - apply IHh with (f := f'); now eauto.
-    - apply H; now auto.
-    - simpl; apply H0; now eauto.
-    - exact step.
-    - reflexivity.
-  Qed.
-
-  (* This should be the strongest postcondition for [While e Do body
-  Done], given P as a precondition. *)
-
-  Inductive invariant : forall (P : pred) (e : expr) (i : insn) (f : env), Prop :=
-  | inv_0 : forall (P : pred) e i f, P f -> invariant P e i f
-  | inv_s : forall (P : pred) e i f g,
-      eval_expr f e <> 0 ->
-      big_step f i g ->
-      invariant P e i f ->
-      invariant P e i g.
-
-  Hint Constructors invariant.
-  
-  Lemma while_SP_1 : forall body e (P : pred) f,
-      P f -> invariant P e body f.
-  Proof.
-    intros; econstructor; now eauto.
-  Qed.
-
-  Lemma while_SP_2_gen : forall body e (P Q : pred),
-      (forall f g, P f -> big_step f (While e Do body Done) g -> Q g) ->
-      forall g h, invariant P e body g -> big_step g (While e Do body Done) h -> Q h.
-  Proof.
-    intros until h; intros inv; induction inv.
-    - intros; eapply H; now eauto.
-    - intros; apply IHinv; auto.
-      econstructor; now eauto.
-  Qed.
-  
-
-  Lemma while_SP_2 : forall body e (P Q : pred),
-      (forall f g, P f -> big_step f (While e Do body Done) g -> Q g) ->
-      forall g, invariant P e body g -> eval_expr g e = 0 -> Q g.
-  Proof.
-    intros; eapply while_SP_2_gen; now eauto.
-  Qed.
-  
-  
-  Theorem hoare_complete : forall i (P Q : pred),
-      (forall f g, P f -> big_step f i g -> Q g) -> hoare P i Q.
-  Proof.
-    induction i; intros P Q prop.
-    - apply H_Weak with (P := P)(Q := P); auto.
-      intros.
-      eapply prop; try apply H; now auto.
-    (* eauto works! *)
-    - apply H_Weak with (P := (fun f => Q (f [s --> eval_expr f e])))(Q := Q); eauto.
-    - apply H_Seq with (Q := fun f => forall g, big_step f i2 g -> Q g).
-      + apply IHi1.
-        intros; eauto.
-      + apply IHi2; intros; eauto.
-    - apply H_Ite.
-      + apply IHi1; intros.
-        eapply prop; destruct H; eauto.
-      + apply IHi2; intros.
-        eapply prop; destruct H; eauto.
-    - eapply H_While with (I := invariant P e i); intros.
-      + apply IHi.
-        intros f g [neq H] bs. now eauto.
-      + eapply while_SP_2; now eauto.
-      + eapply while_SP_1; now eauto.
-  Qed.
