logic.v
@@ -1,0 +1,153 @@
+Require Import String ZArith Lia.
+Require Export lang.
+
+Definition pred := env -> Prop.
+
+Open Scope lang_scope.
+
+(* Extraordinalriy awkward because of higher-order unification...
+   I think this is mostly solved by defining a WP.
+ *)
+Inductive hoare : pred -> insn -> pred -> Prop :=
+| H_Skip : forall P,
+    hoare P Skip P
+| H_Assign : forall P x e,
+    hoare (fun f => P (f [x --> eval_expr f e])) (x :== e) P
+| H_Seq : forall P Q R i j,
+    hoare P i Q ->
+    hoare Q j R ->
+    hoare P (i;j) R
+| H_Ite : forall P Q e i j,
+    hoare (fun f => eval_expr f e <> 0 /\ P f) i Q ->
+    hoare (fun f => eval_expr f e = 0 /\ P f) j Q ->
+    hoare P (If e Then i Else j) Q
+| H_While : forall (P Q I : pred) e i,
+    hoare (fun f => eval_expr f e <> 0 /\ I f) i I ->
+    (forall f, I f -> eval_expr f e = 0 -> Q f) ->
+    (forall f, P f -> I f) ->
+    hoare P (While e Do i Done) Q
+| H_Weak : forall (P P' Q Q' : pred) i,
+    (forall f, P' f -> P f) ->
+    (forall f, Q f -> Q' f) ->
+    hoare P i Q ->
+    hoare P' i Q'
+.
+
+Hint Constructors hoare.
+
+Example test : hoare (fun f => True) ("foo" :== 42) (fun f => f "foo" = 42).
+Proof.
+  eapply H_Weak.
+  - intros.
+    assert (H' : f ["foo" --> eval_expr f 42] "foo" = 42) by reflexivity.
+    exact H'.
+  - intros.
+    exact H.
+  - apply H_Assign with (P := fun f => f "foo" = 42).
+Qed.
+
+Example test' : hoare (fun f => True) (If 0 Then Skip Else "foo" :== 42) (fun f => f "foo" = 42).
+Proof.
+  apply H_Ite.
+  - simpl.
+    apply H_Weak with (P := fun f => f "foo" = 42)(Q := fun f => f "foo" = 42); intros; firstorder.
+  - eapply H_Weak with (P := fun f => f ["foo" --> eval_expr f 42] "foo" = 42)
+                       (Q := fun f => f "foo" = 42).
+    + simpl; now auto.
+    + now auto.
+    + apply H_Assign with (P := fun f => f "foo" = 42).
+Qed.
+
+Lemma while_inv : forall (I Q : pred) i body f g e,
+    (forall f' g', I f' -> eval_expr f' e <> 0 -> big_step f' body g' -> I g') ->
+    (forall f', I f' -> eval_expr f' e = 0 -> Q f') ->
+    I f ->
+    big_step f i g ->
+    (i = While e Do body Done) ->
+    Q g.
+Proof.
+  intros I Q i body f g e inv_body inv_break init big.
+  induction big; intro eq; try inversion eq; subst; auto.
+  apply IHbig2; [| now auto].
+  eapply inv_body; [| apply H | apply big1].
+  apply init.
+Qed.
+
+Theorem hoare_sound : forall f g P Q i,
+    hoare P i Q -> big_step f i g -> P f -> Q g.
+Proof.
+  intros f g P Q i h.
+  revert f g.
+  induction h; intros f g step; inversion step; subst; eauto.
+  (* 1 subgoal! *)
+  intro hf.
+  eapply while_inv; intros.
+  - apply IHh with (f := f'); now eauto.
+  - apply H; now auto.
+  - simpl; apply H0; now eauto.
+  - exact step.
+  - reflexivity.
+Qed.
+
+(* This should be the strongest postcondition for [While e Do body
+  Done], given P as a precondition. *)
+
+Inductive invariant : forall (P : pred) (e : expr) (i : insn) (f : env), Prop :=
+| inv_0 : forall (P : pred) e i f, P f -> invariant P e i f
+| inv_s : forall (P : pred) e i f g,
+    eval_expr f e <> 0 ->
+    big_step f i g ->
+    invariant P e i f ->
+    invariant P e i g.
+
+Hint Constructors invariant.
+
+Lemma while_SP_1 : forall body e (P : pred) f,
+    P f -> invariant P e body f.
+Proof.
+  intros; econstructor; now eauto.
+Qed.
+
+Lemma while_SP_2_gen : forall body e (P Q : pred),
+    (forall f g, P f -> big_step f (While e Do body Done) g -> Q g) ->
+    forall g h, invariant P e body g -> big_step g (While e Do body Done) h -> Q h.
+Proof.
+  intros until h; intros inv; induction inv.
+  - intros; eapply H; now eauto.
+  - intros; apply IHinv; auto.
+    econstructor; now eauto.
+Qed.
+
+
+Lemma while_SP_2 : forall body e (P Q : pred),
+    (forall f g, P f -> big_step f (While e Do body Done) g -> Q g) ->
+    forall g, invariant P e body g -> eval_expr g e = 0 -> Q g.
+Proof.
+  intros; eapply while_SP_2_gen; now eauto.
+Qed.
+
+
+Theorem hoare_complete : forall i (P Q : pred),
+    (forall f g, P f -> big_step f i g -> Q g) -> hoare P i Q.
+Proof.
+  induction i; intros P Q prop.
+  - apply H_Weak with (P := P)(Q := P); auto.
+    intros.
+    eapply prop; try apply H; now auto.
+  (* eauto works! *)
+  - apply H_Weak with (P := (fun f => Q (f [s --> eval_expr f e])))(Q := Q); eauto.
+  - apply H_Seq with (Q := fun f => forall g, big_step f i2 g -> Q g).
+    + apply IHi1.
+      intros; eauto.
+    + apply IHi2; intros; eauto.
+  - apply H_Ite.
+    + apply IHi1; intros.
+      eapply prop; destruct H; eauto.
+    + apply IHi2; intros.
+      eapply prop; destruct H; eauto.
+  - eapply H_While with (I := invariant P e i); intros.
+    + apply IHi.
+      intros f g [neq H] bs. now eauto.
+    + eapply while_SP_2; now eauto.
+    + eapply while_SP_1; now eauto.
+Qed.
