wp.v
@@ -1,0 +1,48 @@
+Require Import String ZArith Lia.
+Require Export logic.
+
+
+(* We need invariants to compute the WP *)
+Definition inv_map := insn -> pred.
+
+Search (Z -> Z -> bool).
+
+Fixpoint wp (inv_map : inv_map) (insn : insn) (post : pred) : pred :=
+  match insn with
+  | Skip => post
+  | x :== e => fun f => post (f [x --> eval_expr f e])
+  | (i1 ; i2) => wp inv_map i1 (wp inv_map i2 post)
+  | If e Then i1 Else i2 =>
+    fun f =>
+      if Zneq_bool (eval_expr f e) 0
+      then wp inv_map i1 post f
+      else wp inv_map i2 post f
+  | (While e Do body Done) =>
+    fun f =>
+      let I := inv_map insn in
+      (forall g, I g -> eval_expr g e = 0 -> post g)
+      /\
+      (* anything about eval_expr f e <> 0? *)
+      I f
+  end.
+
+(* FIXME: this definition... *)
+Definition inv_map_correct (inv_map : inv_map) : Prop :=
+  forall e body,
+    let I := inv_map (While e Do body Done) in
+    hoare (fun f => eval_expr f e <> 0 /\ I f) body I.
+
+Theorem wp_sound : forall inv_map post insn,
+    inv_map_correct inv_map ->
+    hoare (wp inv_map insn post) insn post.                         
+Proof.
+Admitted.
+
+
+
+Theorem wp_complete : forall inv_map pre post insn,
+    inv_map_correct inv_map ->
+    hoare pre insn post ->
+    forall f, pre f -> wp inv_map insn post f.
+Proof.
+Admitted.
